theories/logic/sem_judgement.v
@@ -31,24 +31,24 @@ From haffel.logic Require Import ewpw.
 Definition sem_typed `{!heapGS Σ}
   (Γ₁ : env Σ)
   (e : expr)
-  (σ : sem_sig Σ)
+  (ρ : sem_row Σ)
   (τ : sem_ty Σ) 
   (Γ₂ : env Σ) : iProp Σ :=
     tc_opaque (□ (∀ (vs : gmap string val),
                     env_sem_typed Γ₁ vs -∗ 
-                    (EWPW (subst_map vs e) <| σ |> {{ v, τ v ∗ env_sem_typed Γ₂ vs }})))%I.
+                    (EWPW (subst_map vs e) <| ρ |> {{ v, τ v ∗ env_sem_typed Γ₂ vs }})))%I.
 
-Global Instance sem_typed_persistent `{!heapGS Σ} (Γ Γ' : env Σ) e σ τ :
-  Persistent (sem_typed Γ e σ τ Γ').
+Global Instance sem_typed_persistent `{!heapGS Σ} (Γ Γ' : env Σ) e ρ τ :
+  Persistent (sem_typed Γ e ρ τ Γ').
 Proof.
   unfold sem_typed, tc_opaque. apply _.
 Qed.
 
-Notation "Γ₁ ⊨ e : σ : α ⊨ Γ₂" := (sem_typed Γ₁ e%E σ%S α%T Γ₂)
-  (at level 74, e, σ, α at next level) : bi_scope.
+Notation "Γ₁ ⊨ e : ρ : α ⊨ Γ₂" := (sem_typed Γ₁ e%E ρ%R α%T Γ₂)
+  (at level 74, e, ρ, α at next level) : bi_scope.
 
-Notation "⊨ e : σ : α" := (sem_typed [] e%E σ%S α%T [])
-  (at level 74, e, σ, α at next level) : bi_scope.
+Notation "⊨ e : ρ : α" := (sem_typed [] e%E ρ%R α%T [])
+  (at level 74, e, ρ, α at next level) : bi_scope.
 
 (* The value semantic typing judgement is also defined
  * to be persistent, so only persistent values hold for it.
